Core/Ppcc/Examples.lean
@@ -3,33 +3,3 @@ import Core.Ppcc.Basic
 import Core.Eval
 
 import Core.Infer
-
-namespace Core.EqGraph.Test
-
-def CtxWf : ⊢ [] := by constructor
-
-def mEG1 : Option (Core.Ppcc.EqGraph [] [★, ★, ★, ★] [t#0 ~[★]~ t#1, t#1 ~[★]~ t#2])
-  := Core.Ppcc.EqGraph.process_tyenv (G := []) (Δ := [★, ★, ★, ★]) (wf := CtxWf) (Γ := [t#0 ~[★]~ t#1, t#1 ~[★]~ t#2])
-
-def test1 : Option Ty := do
-  let eG <- mEG1
-  let Δ := [★, ★, ★, ★]
-  let Γ := [t#0 ~[★]~ t#1, t#1 ~[★]~ t#2]
-  let ⟨t, _⟩ <- eG.ask [] CtxWf Δ Γ  ★ t#1 t#2
-  Term.infer_type [] Δ Γ t
-
-#guard test1 == some (t#1 ~[★]~ t#2)
-
-def mEG2 : Option (Core.Ppcc.EqGraph [] [★ -:> ★, ★ -:> ★, ★, ★] [(t#0 • t#2) ~[★]~ (t#1 • t#3)])
-  := Core.Ppcc.EqGraph.process_tyenv [] CtxWf [★ -:> ★, ★ -:> ★, ★, ★] [(t#0 • t#2) ~[★]~ (t#1 • t#3)]
-
-def test2 : Option Ty := do
-  let eG <- mEG2
-  let Δ := [★ -:> ★, ★ -:> ★, ★, ★]
-  let Γ := [(t#0 • t#2) ~[★]~ (t#1 • t#3)]
-  let ⟨t, _⟩ <- eG.ask [] CtxWf Δ Γ (★ -:> ★) t#0 t#1
-  Term.infer_type [] Δ Γ t
-
-#guard test2 == some (t#0 ~[★ -:> ★]~ t#1)
-
-end Core.EqGraph.Test
