Core/Ppcc/Lemmas.lean
@@ -11,14 +11,4 @@ theorem EqGraph.ask_type_sound {G : GlobalEnv} {wf : ⊢ G} {Δ : KindEnv} {Γ :
   G&Δ, Γ ⊢ c : (T1 ~[K]~ T2) :=
   by intro h; apply j
 
-
-theorem env_consistency {G : GlobalEnv} {wf : ⊢ G} {Δ : KindEnv} {Γ : TyEnv} :
-  TyEnv.is_consistent G wf Δ Γ = some () ->
-  ∀ T1 T2 K, T1 ≠ T2 -> ¬ (G&Δ, Γ ⊢ c : (gt#T1 ~[K]~ gt#T2))
-:= by
- intro h T1 T2 K ne j
- unfold TyEnv.is_consistent at h; simp at h
-
- sorry
-
 end Core.Ppcc
